some refactoring of the soundness module

examples/dsls/mini_steel/Pulse.Soundness.Exists.fsti
@@ -1,102 +1,41 @@
 module Pulse.Soundness.Exists
 
-open FStar.Reflection
-open Pulse.Reflection.Util
+open Pulse.Syntax
+open Pulse.Typing
+open Pulse.Elaborate.Pure
+open Pulse.Elaborate.Core
+open Pulse.Soundness.Common
 
 module RT = Refl.Typing
 
-val exists_inversion
+val intro_exists_erased_soundness
+  (#f:stt_env)
   (#g:env)
-  (#u:universe)
-  (#a:term)
-  (#p:term)
-  (e_typing:RT.typing g
-                      (mk_exists u a p)
-                      vprop_tm)
-  : GTot (RT.typing g
-                    p
-                   (mk_arrow (a, Q_Explicit) vprop_tm))
+  (#t:st_term)
+  (#c:comp)
+  (d:st_typing f g t c{T_IntroExistsErased? d})
+  : GTot (RT.typing (extend_env_l f g)
+                    (elab_st_typing d)
+                    (elab_comp c))
 
-(*
-
- g |- a : Type u
- g |- p : a -> vprop
- ----------------------------------------------------------------
- g |- elim_exists<u> #a p : stt_ghost<u> a empty (exists_<u> p) (fun x -> p (reveal x))
-
-*)
-
-let elim_exists_post_body (u:universe) (a:term) (p:term) (x:var) =
-  let x_tm = RT.var_as_term x in
-  let reveal_x = mk_reveal u a x_tm in
-  let post = pack_ln (Tv_App p (reveal_x, Q_Explicit)) in
-  RT.open_or_close_term' post (RT.CloseVar x) 0
-
-let elim_exists_post (u:universe) (a:term) (p:term) (x:var) =
-  let erased_a = mk_erased u a in
-  mk_abs erased_a Q_Explicit (elim_exists_post_body u a p x)
+val intro_exists_soundness
+  (#f:stt_env)
+  (#g:env)
+  (#t:st_term)
+  (#c:comp)
+  (d:st_typing f g t c{T_IntroExists? d })
+  : GTot (RT.typing (extend_env_l f g)
+                    (elab_st_typing d)
+                    (elab_comp c))
 
 val elim_exists_soundness
+  (#f:stt_env)
   (#g:env)
-  (#u:universe)
-  (#a:term)
-  (#p:term)
-  (x:var{None? (RT.lookup_bvar g x)})
-  (a_typing:RT.typing g a (pack_ln (Tv_Type u)))
-  (p_typing:RT.typing g p (mk_arrow (a, Q_Explicit) vprop_tm))
-  : GTot (RT.typing g
-                 (mk_elim_exists u a p)
-                 (mk_stt_ghost_comp
-                    u
-                    (mk_erased u a) 
-                    emp_inames_tm
-                    (mk_exists u a p)
-                    (elim_exists_post u a p x)))
+  (#t:st_term)
+  (#c:comp)
+  (d:st_typing f g t c{T_ElimExists? d})
+  : GTot (RT.typing (extend_env_l f g)
+                    (elab_st_typing d)
+                    (elab_comp c))
 
-(*
 
- g |- a : Type u
- g |- p : a -> vprop
- g |- e : vprop
- -------------------------------------------------------------------------
- g |- intro_exists<u> #a p e : stt_ghost<0> unit empty (p e) (fun _ -> exists_ p)
-
-*)
-val intro_exists_soundness
-  (#g:env)
-  (#u:universe)
-  (#a:term)
-  (#p:term)
-  (#e:term)
-  (a_typing:RT.typing g a (pack_ln (Tv_Type u)))
-  (p_typing:RT.typing g p (mk_arrow (a, Q_Explicit) vprop_tm))
-  (e_typing:RT.typing g e a)
-  : GTot (RT.typing g
-                 (mk_intro_exists u a p e)
-                 (mk_stt_ghost_comp uzero unit_tm emp_inames_tm
-                    (pack_ln (Tv_App p (e, Q_Explicit)))
-                    (mk_abs unit_tm Q_Explicit (mk_exists u a p))))
-
-(*
-
- g |- a : Type u
- g |- p : a -> vprop
- g |- e : vprop
- -------------------------------------------------------------------------
- g |- intro_exists<u> #a p e : stt_ghost<0> unit empty (p e) (fun _ -> exists_ p)
-
-*)
-val intro_exists_erased_soundness
-  (#g:env)
-  (#u:universe)
-  (#a:term)
-  (#p:term)
-  (#e:term)
-  (a_typing:RT.typing g a (pack_ln (Tv_Type u)))
-  (p_typing:RT.typing g p (mk_arrow (a, Q_Explicit) vprop_tm))
-  (e_typing:RT.typing g e (mk_erased u a))
-  : GTot (RT.typing g
-                 (mk_intro_exists_erased u a p e)
-                 (mk_stt_ghost_comp uzero unit_tm emp_inames_tm
-                    (pack_ln (Tv_App p (mk_reveal u a e, Q_Explicit)))
-                    (mk_abs unit_tm Q_Explicit (mk_exists u a p))))
