examples/dsls/mini_steel/Pulse.Soundness.fst
@@ -19,49 +19,14 @@ module Exists = Pulse.Soundness.Exists
 module While = Pulse.Soundness.While
 module Admit = Pulse.Soundness.Admit
 module Par = Pulse.Soundness.Par
+module Comp = Pulse.Soundness.Comp
 module LN = Pulse.Typing.LN
 module FV = Pulse.Typing.FV
 module STT = Pulse.Soundness.STT
 
 module Typing = Pulse.Typing
 module EPure = Pulse.Elaborate.Pure
-
-let elab_open_commute' (e:term) (v:term) (n:index)
-  : Lemma (ensures
-             RT.open_or_close_term' (elab_term e) (RT.OpenWith (elab_term v)) n ==
-             elab_term (open_term' e v n))
-          [SMTPat (elab_term (open_term' e v n))] =
-
-  elab_open_commute' e v n
-
-let elab_close_commute' (e:term) (v:var) (n:index)
-  : Lemma (RT.open_or_close_term' (elab_term e) (RT.CloseVar v) n ==
-           elab_term (close_term' e v n))
-          [SMTPat (elab_term (close_term' e v n))] =
-
-  elab_close_commute' e v n
-
-let elab_comp_close_commute (c:comp) (x:var)
-  : Lemma (ensures elab_comp (close_comp c x) == RT.close_term (elab_comp c) x)
-          [SMTPat (elab_comp (close_comp c x))] =
-
-  elab_comp_close_commute c x
-
-let elab_comp_open_commute (c:comp) (x:term)
-  : Lemma (ensures elab_comp (open_comp_with c x) == RT.open_with (elab_comp c) (elab_term x))
-          [SMTPat (elab_comp (open_comp_with c x))] =
-
-  elab_comp_open_commute c x
-
-let soundness_t (d:'a) = 
-    f:stt_env ->
-    g:env ->
-    t:st_term ->
-    c:comp ->
-    d':st_typing f g t c{d' << d} ->
-    GTot (RT.typing (extend_env_l f g)
-                    (elab_st_typing d')
-                    (elab_comp c))
+module WT= Pulse.Steel.Wrapper.Typing
 
 let tabs_t (d:'a) = 
     #f:stt_env ->
@@ -199,197 +164,6 @@ let bind_soundness
            (tot_typing_soundness reveal_b_typing)
 #pop-options
 
-#push-options "--fuel 4 --ifuel 1"
-let intro_exists_erased_soundness
-  (#f:stt_env)
-  (#g:env)
-  (#t:st_term)
-  (#c:comp)
-  (d:st_typing f g t c{T_IntroExistsErased? d})
-  : GTot (RT.typing (extend_env_l f g)
-                    (elab_st_typing d)
-                    (elab_comp c)) =
-  let t0 = t in
-  let T_IntroExistsErased _ u t p e t_typing p_typing e_typing = d in
-  let ru = elab_universe u in
-  let rt = elab_term t in
-  let rp = elab_term p in
-  let re = elab_term e in
-  let rt_typing : RT.typing _ rt (R.pack_ln (R.Tv_Type ru)) =
-      tot_typing_soundness t_typing in
-
-  let rp_typing
-      : RT.typing _
-                  (mk_exists ru rt (mk_abs rt R.Q_Explicit rp)) vprop_tm =
-      tot_typing_soundness p_typing
-  in
-  let rp_typing
-      : RT.typing _
-                  (mk_abs rt R.Q_Explicit rp)
-                  (mk_arrow (rt, R.Q_Explicit) vprop_tm) =
-        Exists.exists_inversion rp_typing
-  in
-  let re_typing : RT.typing _ re _ =
-      tot_typing_soundness e_typing
-  in
-  let reveal_re = elab_term (mk_reveal u t e) in
-
-  // reveal_re is ln
-  LN.tot_typing_ln e_typing;
-  elab_ln (mk_reveal u t e) (-1);
-
-  //rp is (ln' 0)
-  LN.tot_typing_ln p_typing;
-  elab_ln p 0;
-  
-  RT.beta_reduction rt R.Q_Explicit rp reveal_re;    
-
-  Exists.intro_exists_erased_soundness rt_typing rp_typing re_typing
-
-let intro_exists_soundness
-  (#f:stt_env)
-  (#g:env)
-  (#t:st_term)
-  (#c:comp)
-  (d:st_typing f g t c{T_IntroExists? d })
-  : GTot (RT.typing (extend_env_l f g)
-                    (elab_st_typing d)
-                    (elab_comp c)) =
-
-  let t0 = t in
-  let T_IntroExists _ u t p e t_typing p_typing e_typing = d in
-  let ru = elab_universe u in
-  let rt = elab_term t in
-  let rp = elab_term p in
-  let re = elab_term e in
-  let rt_typing : RT.typing _ rt (R.pack_ln (R.Tv_Type ru)) =
-      tot_typing_soundness t_typing in
-  let rp_typing
-      : RT.typing _
-                  (mk_exists ru rt (mk_abs rt R.Q_Explicit rp)) vprop_tm =
-      tot_typing_soundness p_typing in
-  let rp_typing
-      : RT.typing _
-                  (mk_abs rt R.Q_Explicit rp)
-                  (mk_arrow (rt, R.Q_Explicit) vprop_tm) =
-        Exists.exists_inversion rp_typing
-  in
-  let re_typing : RT.typing _ re _ =
-      tot_typing_soundness e_typing
-  in
-
-  // re is ln
-  LN.tot_typing_ln e_typing;
-  elab_ln e (-1);
-
-  //rp is (ln' 0)
-  LN.tot_typing_ln p_typing;
-  elab_ln p 0;
-
-  RT.beta_reduction rt R.Q_Explicit rp re;
-
-  Exists.intro_exists_soundness rt_typing rp_typing re_typing
-#pop-options
-
-#push-options "--z3rlimit_factor 8 --fuel 4 --ifuel 2"
-let elim_exists_soundness
-  (#f:stt_env)
-  (#g:env)
-  (#t:st_term)
-  (#c:comp)
-  (d:st_typing f g t c{T_ElimExists? d})
-  : GTot (RT.typing (extend_env_l f g)
-                    (elab_st_typing d)
-                    (elab_comp c)) =
-
-  let T_ElimExists _ u t p x t_typing p_typing = d in
-  let ru = elab_universe u in
-  let rt = elab_term t in
-  let rp = elab_term p in
-  let rt_typing = tot_typing_soundness t_typing in
-  let rp_typing
-    : RT.typing (extend_env_l f g)
-                (mk_exists ru (elab_term t)
-                   (mk_abs (elab_term t) R.Q_Explicit (elab_term p)))
-                vprop_tm
-    = tot_typing_soundness p_typing in
-  let rp_typing = Exists.exists_inversion rp_typing in
-
-  FV.st_typing_freevars_inv d x;
-  assert (~ (Set.mem x (freevars t)));
-  assert (~ (Set.mem x (freevars p)));
-
-  let x_tm = Tm_Var {nm_index=x;nm_ppname=RT.pp_name_default} in
-  let rx_tm = R.pack_ln (R.Tv_Var (R.pack_bv (RT.make_bv x tun))) in
-  let rx_bv = R.pack_ln (R.Tv_BVar (R.pack_bv (RT.make_bv 0 tun))) in
-
-  // rt is ln
-  LN.tot_typing_ln t_typing;
-  elab_ln t (-1);
-
-  //rp is (ln' 0)
-  LN.tot_typing_ln p_typing;
-  elab_ln p 0;
-
-  calc (==) {
-    elab_term (close_term' (open_term' p (mk_reveal u t x_tm) 0) x 0);
-       (==) {
-               RT.beta_reduction rt R.Q_Explicit rp (Pulse.Reflection.Util.mk_reveal ru rt rx_tm)
-            }
-    Exists.elim_exists_post_body ru rt (mk_abs rt R.Q_Explicit rp) x;
-  };
-  Exists.elim_exists_soundness x rt_typing rp_typing
-#pop-options
-
-#push-options "--z3rlimit_factor 4 --fuel 4 --ifuel 2"
-let while_soundness
-  (#f:stt_env)
-  (#g:env)
-  (#t:st_term)
-  (#c:comp)
-  (d:st_typing f g t c{T_While? d})
-  (soundness: soundness_t d)
-  : GTot (RT.typing (extend_env_l f g)
-                    (elab_st_typing d)
-                    (elab_comp c)) =
-
-  let T_While _ inv cond body inv_typing cond_typing body_typing = d in
-  let rinv = mk_abs bool_tm R.Q_Explicit (elab_term inv) in
-  let rinv_typing
-    : RT.typing _
-        (mk_exists uzero bool_tm rinv)
-        vprop_tm =
-    tot_typing_soundness inv_typing in
-  let rinv_typing
-    : RT.typing _
-        rinv
-        (mk_arrow (bool_tm, R.Q_Explicit) vprop_tm) =
-    Exists.exists_inversion rinv_typing in
-  let rcond_typing
-    : RT.typing _ (elab_st_typing cond_typing)
-        (mk_stt_comp uzero bool_tm (mk_exists uzero bool_tm rinv) rinv) =
-    soundness f g cond (comp_while_cond inv) cond_typing in
-
-  // (elab_term inv) is (ln 0)
-  LN.tot_typing_ln inv_typing;
-  elab_ln inv 0;
-
-  elab_open_commute' inv tm_true 0;
-  RT.beta_reduction bool_tm R.Q_Explicit (elab_term inv) true_tm;
-
-  let rbody_typing
-    : RT.typing _ (elab_st_typing body_typing)
-        (mk_stt_comp uzero unit_tm
-           (R.pack_ln (R.Tv_App rinv (true_tm, R.Q_Explicit)))
-           (mk_abs unit_tm R.Q_Explicit (mk_exists uzero bool_tm rinv))) =
-    soundness f g body (comp_while_body inv) body_typing in
-
-  elab_open_commute' inv tm_false 0;
-  RT.beta_reduction bool_tm R.Q_Explicit (elab_term inv) false_tm;
-
-  While.while_soundness rinv_typing rcond_typing rbody_typing
-#pop-options
-
 #push-options "--z3rlimit_factor 4 --fuel 4 --ifuel 2"
 let if_soundness
   (f:stt_env)
@@ -443,228 +217,6 @@ let if_soundness
   RT.T_If _ _ _ _ _ _ _ rb_typing re1_typing re2_typing c_typing
 #pop-options
 
-let stc_soundness
-  (#f:stt_env)
-  (#g:env)
-  (#st:st_comp)
-  (d_st:st_comp_typing f g st)
-  
-  : GTot (RT.typing (extend_env_l f g)
-                    (elab_term st.res)
-                    (RT.tm_type (elab_universe st.u)) &
-          RT.typing (extend_env_l f g)
-                    (elab_term st.pre)
-                    vprop_tm &
-          RT.typing (extend_env_l f g)
-                    (mk_abs (elab_term st.res) R.Q_Explicit
-                                                   (elab_term st.post))
-                    (post1_type_bind (elab_term st.res))) =
-   
-  let STC _ st x dres dpre dpost = d_st in
-  let res_typing = tot_typing_soundness dres in
-  let pre_typing = tot_typing_soundness dpre in      
-  calc (==) {
-    RT.close_term (elab_term (open_term st.post x)) x;
-       (==) { elab_open_commute st.post x }
-    RT.close_term (RT.open_term (elab_term st.post) x) x;
-       (==) { 
-              elab_freevars st.post;
-              RT.close_open_inverse (elab_term st.post) x
-            }
-    elab_term st.post;
-  };
-  let post_typing  = mk_t_abs_tot f g RT.pp_name_default dres dpost in
-  res_typing, pre_typing, post_typing
-
-#push-options "--query_stats --fuel 2 --ifuel 2 --z3rlimit_factor 2"
-let comp_typing_soundness (f:stt_env)
-                          (g:env)
-                          (c:comp)
-                          (uc:universe)
-                          (d:comp_typing f g c uc)
-  : GTot (RT.typing (extend_env_l f g) (elab_comp c) (RT.tm_type (elab_universe uc)))
-         (decreases d)
-  = match d with
-    | CT_Tot _ t _ dt ->
-      tot_typing_soundness dt
-      
-    | CT_ST _ st d_st -> 
-      let res_typing, pre_typing, post_typing = stc_soundness d_st in
-      STT.stt_typing res_typing pre_typing post_typing
-
-    | CT_STAtomic _ i st d_i d_st -> 
-      let i_typing = tot_typing_soundness d_i in
-      let res_typing, pre_typing, post_typing = stc_soundness d_st in
-      STT.stt_atomic_typing res_typing i_typing pre_typing post_typing
-
-    | CT_STGhost _ i st d_i d_st -> 
-      let i_typing = tot_typing_soundness d_i in
-      let res_typing, pre_typing, post_typing = stc_soundness d_st in
-      STT.stt_ghost_typing res_typing i_typing pre_typing post_typing
-#pop-options
-
-let admit_soundess
-  (#f:stt_env)
-  (#g:env)
-  (#t:st_term)
-  (#c:comp)
-  (d:st_typing f g t c{T_Admit? d})
-  : GTot (RT.typing (extend_env_l f g)
-                    (elab_st_typing d)
-                    (elab_comp c)) =
-
-  let T_Admit _ s c st_typing = d in
-
-  let rt_typing, rpre_typing, rpost_typing = stc_soundness st_typing in
-  match c with
-  | STT ->
-    Admit.stt_admit_soundness rt_typing rpre_typing rpost_typing
-  | STT_Atomic ->
-    Admit.stt_atomic_admit_soundness rt_typing rpre_typing rpost_typing
-  | STT_Ghost ->
-    Admit.stt_ghost_admit_soundness rt_typing rpre_typing rpost_typing
-
-#push-options "--z3rlimit_factor 10 --fuel 4 --ifuel 2"
-let return_soundess
-  (#f:stt_env)
-  (#g:env)
-  (#t:st_term)
-  (#c:comp)
-  (d:st_typing f g t c{T_Return? d})
-  : GTot (RT.typing (extend_env_l f g)
-                    (elab_st_typing d)
-                    (elab_comp c)) =
-
-  let T_Return _ ctag use_eq u t e post x t_typing e_typing post_typing = d in
-  let ru = elab_universe u in
-  let rt = elab_term t in
-  let re = elab_term e in
-  let rpost = elab_term post in
-  let rpost = mk_abs rt R.Q_Explicit rpost in
-  let rt_typing : RT.typing _ rt (R.pack_ln (R.Tv_Type ru)) =
-    tot_typing_soundness t_typing in
-  let re_typing : RT.typing _ re rt =
-    tot_typing_soundness e_typing in
-  let rpost_typing
-    : RT.typing _ rpost
-                  (mk_arrow (rt, R.Q_Explicit) vprop_tm) =
-    mk_t_abs_tot f g RT.pp_name_default t_typing post_typing in
-
-  // re is ln
-  LN.tot_typing_ln e_typing;
-  elab_ln e (-1);
-
-  // (elab_term post) is (ln 0)
-  RT.well_typed_terms_are_ln _ rpost _ rpost_typing;
-  assert (RT.ln' (elab_term post) 0);
-
-  elab_open_commute' post e 0;
-  RT.beta_reduction rt R.Q_Explicit (elab_term post) re;
-  
-  match ctag, use_eq with
-  | STT, true ->
-    Return.return_stt_typing x rt_typing re_typing rpost_typing
-  | STT, false -> 
-    Return.return_stt_noeq_typing rt_typing re_typing rpost_typing
-  | STT_Atomic, true ->
-    Return.return_stt_atomic_typing x rt_typing re_typing rpost_typing
-  | STT_Atomic, false -> 
-    Return.return_stt_atomic_noeq_typing rt_typing re_typing rpost_typing
-  | STT_Ghost, true ->
-    Return.return_stt_ghost_typing x rt_typing re_typing rpost_typing
-  | STT_Ghost, false -> 
-    Return.return_stt_ghost_noeq_typing rt_typing re_typing rpost_typing
-#pop-options
-
-#push-options "--z3rlimit_factor 10 --fuel 8 --ifuel 1"
-let par_soundness
-  (#f:stt_env)
-  (#g:env)
-  (#t:st_term)
-  (#c:comp)
-  (d:st_typing f g t c{T_Par? d})
-  (soundness: soundness_t d)
-  : GTot (RT.typing (extend_env_l f g)
-                    (elab_st_typing d)
-                    (elab_comp c)) =
-
-  let T_Par _ eL cL eR cR x cL_typing cR_typing eL_typing eR_typing = d in
-
-  let ru = elab_universe (comp_u cL) in
-  let raL = elab_term (comp_res cL) in
-  let raR = elab_term (comp_res cR) in
-  let rpreL = elab_term (comp_pre cL) in
-  let rpostL = mk_abs raL R.Q_Explicit (elab_term (comp_post cL)) in
-  let rpreR = elab_term (comp_pre cR) in
-  let rpostR = mk_abs raR R.Q_Explicit (elab_term (comp_post cR)) in
-  let reL = elab_st_typing eL_typing in
-  let reR = elab_st_typing eR_typing in
-
-  let reL_typing
-    : RT.typing _ reL (elab_comp cL) =
-    soundness f g eL cL eL_typing in
-
-  let reR_typing
-    : RT.typing _ reR (elab_comp cR) =
-    soundness f g eR cR eR_typing in
-
-  let (raL_typing, rpreL_typing, rpostL_typing)
-    : (RT.typing _ raL (R.pack_ln (R.Tv_Type ru)) &
-       RT.typing _ rpreL vprop_tm &
-       RT.typing _ rpostL (mk_arrow (raL, R.Q_Explicit) vprop_tm)) =
-
-    inversion_of_stt_typing f g cL ru (comp_typing_soundness f g cL (comp_u cL) cL_typing) in
-
-  let (raR_typing, rpreR_typing, rpostR_typing)
-    : (RT.typing _ raR (R.pack_ln (R.Tv_Type ru)) &
-       RT.typing _ rpreR vprop_tm &
-       RT.typing _ rpostR (mk_arrow (raR, R.Q_Explicit) vprop_tm)) =
-
-    inversion_of_stt_typing f g cR ru (comp_typing_soundness f g cR (comp_u cR) cR_typing) in
-
-  /////
-  let uL = comp_u cL in
-  let uR = comp_u cR in
-  let aL = comp_res cL in
-  let aR = comp_res cR in
-  let postL = comp_post cL in
-  let postR = comp_post cR in
-  let x_tm = term_of_var x in
-
-  // ln proofs for invoking the RT beta reduction
-  RT.well_typed_terms_are_ln _ _ _ raL_typing;
-  RT.well_typed_terms_are_ln _ _ _ raR_typing;
-  RT.well_typed_terms_are_ln _ _ _ rpostL_typing;
-  RT.well_typed_terms_are_ln _ _ _ rpostR_typing;
-
-  calc (==) {
-    elab_term (par_post uL uR aL aR postL postR x);
-       (==) { }
-    RT.open_or_close_term'
-      (mk_star
-         (RT.open_or_close_term'
-            (elab_term postL)
-            (RT.OpenWith (elab_term (mk_fst uL uR aL aR x_tm))) 0)
-         (RT.open_or_close_term'
-            (elab_term postR)
-            (RT.OpenWith (elab_term (mk_snd uL uR aL aR x_tm))) 0))
-      (RT.CloseVar x)
-      0;
-       (==) { RT.beta_reduction raL R.Q_Explicit
-                (elab_term postL)
-                (Pulse.Reflection.Util.mk_fst ru ru raL raR (RT.var_as_term x));
-              RT.beta_reduction raR R.Q_Explicit
-                (elab_term postR)
-                (Pulse.Reflection.Util.mk_snd ru ru raL raR (RT.var_as_term x)) }
-    Par.par_post ru raL raR rpostL rpostR x;
-  };
-  /////
-
-  Par.par_soundness x raL_typing raR_typing rpreL_typing rpostL_typing
-    rpreR_typing rpostR_typing
-    reL_typing reR_typing
-#pop-options
-
 #push-options "--query_stats --fuel 2 --ifuel 2"
 let rec soundness (f:stt_env)
                   (g:env)
@@ -714,30 +266,30 @@ let rec soundness (f:stt_env)
       stequiv_soundness _ _ _ _ d soundness
 
     | T_Return _ _ _ _ _ _ _ _ _ _ _ ->
-      return_soundess d
+      Return.return_soundess d
 
     | T_If _ _ _ _ _ _ _ _ _ _ _->
       let ct_soundness f g c uc (d':_ {d' << d}) =
-        comp_typing_soundness f g c uc d'
+        Comp.comp_typing_soundness f g c uc d'
       in
       if_soundness _ _ _ _ d soundness ct_soundness
 
     | T_ElimExists _ _ _ _ _ _ _ ->
-      elim_exists_soundness d
+      Exists.elim_exists_soundness d
 
     | T_IntroExists _ _ _ _ _ _ _ _ ->
-      intro_exists_soundness d
+      Exists.intro_exists_soundness d
 
     | T_IntroExistsErased _ _ _ _ _ _ _ _ ->
-      intro_exists_erased_soundness d
+      Exists.intro_exists_erased_soundness d
 
     | T_While _ _ _ _ _ _ _ ->
-      while_soundness d soundness
+      While.while_soundness d soundness
 
     | T_Par _ _ _ _ _ _ _ _ _ _ ->
-      par_soundness d soundness
+      Par.par_soundness d soundness
 
-    | T_Admit _ _ _ _ -> admit_soundess d
+    | T_Admit _ _ _ _ -> Admit.admit_soundess d
 #pop-options
 
 let soundness_lemma
