examples/dsls/mini_steel/Pulse.Soundness.Comp.fsti
@@ -1,0 +1,35 @@
+module Pulse.Soundness.Comp
+
+open Pulse.Syntax
+open Pulse.Reflection.Util
+open Pulse.Typing
+open Pulse.Elaborate.Pure
+open Pulse.Elaborate.Core
+open Pulse.Soundness.Common
+
+module R = FStar.Reflection
+module RT = Refl.Typing
+
+val stc_soundness
+  (#f:stt_env)
+  (#g:env)
+  (#st:st_comp)
+  (d_st:st_comp_typing f g st)
+  
+  : GTot (RT.typing (extend_env_l f g)
+                    (elab_term st.res)
+                    (RT.tm_type (elab_universe st.u)) &
+          RT.typing (extend_env_l f g)
+                    (elab_term st.pre)
+                    vprop_tm &
+          RT.typing (extend_env_l f g)
+                    (mk_abs (elab_term st.res) R.Q_Explicit
+                                                   (elab_term st.post))
+                    (post1_type_bind (elab_term st.res)))
+
+val comp_typing_soundness (f:stt_env)
+                          (g:env)
+                          (c:comp)
+                          (uc:universe)
+                          (d:comp_typing f g c uc)
+  : GTot (RT.typing (extend_env_l f g) (elab_comp c) (RT.tm_type (elab_universe uc)))
