examples/dsls/mini_steel/Pulse.Soundness.While.fst
@@ -1,3 +1,64 @@
 module Pulse.Soundness.While
 
-let while_soundness _ _ _ = admit ()
+module R = FStar.Reflection
+module RT = Refl.Typing
+
+open Pulse.Syntax
+open Pulse.Reflection.Util
+open Pulse.Typing
+open Pulse.Elaborate.Pure
+open Pulse.Elaborate.Core
+open Pulse.Elaborate
+open Pulse.Soundness.Common
+
+module WT = Pulse.Steel.Wrapper.Typing
+module LN = Pulse.Typing.LN
+
+#push-options "--z3rlimit_factor 4 --fuel 4 --ifuel 2"
+let while_soundness
+  (#f:stt_env)
+  (#g:env)
+  (#t:st_term)
+  (#c:comp)
+  (d:st_typing f g t c{T_While? d})
+  (soundness: soundness_t d)
+  : GTot (RT.typing (extend_env_l f g)
+                    (elab_st_typing d)
+                    (elab_comp c)) =
+
+  let T_While _ inv cond body inv_typing cond_typing body_typing = d in
+  let rinv = mk_abs bool_tm R.Q_Explicit (elab_term inv) in
+  let rinv_typing
+    : RT.typing _
+        (mk_exists uzero bool_tm rinv)
+        vprop_tm =
+    tot_typing_soundness inv_typing in
+  let rinv_typing
+    : RT.typing _
+        rinv
+        (mk_arrow (bool_tm, R.Q_Explicit) vprop_tm) =
+    WT.exists_inversion rinv_typing in
+  let rcond_typing
+    : RT.typing _ (elab_st_typing cond_typing)
+        (mk_stt_comp uzero bool_tm (mk_exists uzero bool_tm rinv) rinv) =
+    soundness f g cond (comp_while_cond inv) cond_typing in
+
+  // (elab_term inv) is (ln 0)
+  LN.tot_typing_ln inv_typing;
+  elab_ln inv 0;
+
+  elab_open_commute' inv tm_true 0;
+  RT.beta_reduction bool_tm R.Q_Explicit (elab_term inv) true_tm;
+
+  let rbody_typing
+    : RT.typing _ (elab_st_typing body_typing)
+        (mk_stt_comp uzero unit_tm
+           (R.pack_ln (R.Tv_App rinv (true_tm, R.Q_Explicit)))
+           (mk_abs unit_tm R.Q_Explicit (mk_exists uzero bool_tm rinv))) =
+    soundness f g body (comp_while_body inv) body_typing in
+
+  elab_open_commute' inv tm_false 0;
+  RT.beta_reduction bool_tm R.Q_Explicit (elab_term inv) false_tm;
+
+  WT.while_typing rinv_typing rcond_typing rbody_typing
+#pop-options
